# baseURI: http://www.assero.co.uk/ISO11179Identification
# imports: http://purl.org/dc/elements/1.1/
# imports: http://purl.org/dc/terms/
# imports: http://www.w3.org/2004/02/skos/core

@prefix : <http://www.assero.co.uk/ISO11179Identification#> .
@prefix owl: <http://www.w3.org/2002/07/owl#> .
@prefix rdf: <http://www.w3.org/1999/02/22-rdf-syntax-ns#> .
@prefix rdfs: <http://www.w3.org/2000/01/rdf-schema#> .
@prefix skos: <http://www.w3.org/2004/02/skos/core#> .
@prefix xsd: <http://www.w3.org/2001/XMLSchema#> .

<http://www.assero.co.uk/ISO11179Identification>
  rdf:type owl:Ontology ;
  owl:versionInfo "v3.2.0"^^xsd:string ;
  rdfs:label "ISO11179 Identification Schema"^^xsd:string ;
  owl:imports <http://www.w3.org/2004/02/skos/core> ;
.
:Namespace
  rdf:type owl:Class ;
  rdfs:label "Namespace"^^xsd:string ;
  rdfs:subClassOf owl:Thing ;
  skos:definition "A unique framework of authority within which individuals act, or are designated to act, towards some purpose. A scope."^^xsd:string ;
.
:authority
  rdf:type owl:DatatypeProperty ;
  rdfs:domain :Namespace ;
  rdfs:label "Name"^^xsd:string ;
  rdfs:range xsd:string ;
  skos:definition "The authority element of the uri forming the unique string that identifies the namespace."^^xsd:string ;
.
:name
  rdf:type owl:DatatypeProperty ;
  rdfs:domain :Namespace ;
  rdfs:label "Name"^^xsd:string ;
  rdfs:range xsd:string ;
  skos:definition "The full name of the organization (Note: ISO11179 defines this as a 'sign' type, not string)"^^xsd:string ;
.
:shortName
  rdf:type owl:DatatypeProperty ;
  rdfs:domain :Namespace ;
  rdfs:label "Name"^^xsd:string ;
  rdfs:range xsd:string ;
  skos:definition "The short name of the organization."^^xsd:string ;
.
:ScopedIdentifier
  rdf:type owl:Class ;
  rdfs:label "Scoped identifier"^^xsd:string ;
  rdfs:subClassOf owl:Thing ;
  skos:definition "An identifier within a particular scope."^^xsd:string ;
.
:identifier
  rdf:type owl:DatatypeProperty ;
  rdfs:domain :ScopedIdentifier ;
  rdfs:label "identifier"^^xsd:string ;
  rdfs:range xsd:string ;
  skos:definition "String used to unambiguously denote an IdentifiedItem within the scope of a specified Namespace."^^xsd:string ;
.
:version
  rdf:type owl:DatatypeProperty ;
  rdfs:domain :ScopedIdentifier ;
  rdfs:label "Version"^^xsd:string ;
  rdfs:range xsd:positiveInteger ;
  skos:definition "Unique version identifier of the ScopedIdentifier which identifies an IdentifiedItem. Used by the repository to manage versions"^^xsd:string ;
.
:semanticVersion
  rdf:type owl:DatatypeProperty ;
  rdfs:domain :ScopedIdentifier ;
  rdfs:label "Semantic Version"^^xsd:string ;
  rdfs:range xsd:string ;
  skos:definition "Semantic version for the item. Used by the repository to display to users."^^xsd:string ;
.
:versionLabel
  rdf:type owl:DatatypeProperty ;
  rdfs:domain :ScopedIdentifier ;
  rdfs:label "Version Label"^^xsd:string ;
  rdfs:range xsd:string ;
  skos:definition "Human readable version label usually set by external organizations."^^xsd:string ;
.
:hasScope
  rdf:type owl:ObjectProperty ;
  rdfs:domain :ScopedIdentifier ;
  rdfs:label "Scope Relationship"^^xsd:string ;
  rdfs:range :Namespace ;
  skos:definition "The namespce by which this identifier is scoped, i.e. is unique."^^xsd:string ;
